steel/apps/kvstore/Zeta.KeyValueStore.Formats.Spec.fsti
@@ -8,9 +8,63 @@ val key_spec_parser : P.spec_parser key_t
 
 val key_spec_serializer : P.spec_serializer key_spec_parser
 
+val key_spec_parser_injective (b1 b2: _) : Lemma
+  (requires (match key_spec_parser b1, key_spec_parser b2 with
+  | Some (v1, n1), Some (v2, n2) -> v1 == v2
+  | _ -> False
+  ))
+  (ensures (match key_spec_parser b1, key_spec_parser b2 with
+  | Some (v1, n1), Some (v2, n2) -> (n1 <: nat) == n2 /\ Seq.slice b1 0 n1 == Seq.slice b2 0 n2
+  | _ -> True
+  ))
+
+val key_spec_parser_strong_prefix (b1 b2: _) : Lemma
+  (requires (
+    match key_spec_parser b1 with
+    | Some (_, n1) -> n1 <= Seq.length b2 /\ Seq.slice b1 0 n1 == Seq.slice b2 0 n1
+    | _ -> False
+  ))
+  (ensures (
+    match key_spec_parser b1, key_spec_parser b2 with
+    | Some (v1, _), Some (v2, _) -> v1 == v2
+    | _ -> False
+  ))
+
+/// This is an ad hoc bound due to a bound on Blake hashable inputs
+/// FIXME: this bound is necessary because QuackyDucky expects a constant bound on abstract types
+val serialized_key_length (v:key_t)
+  : Lemma (Seq.length (key_spec_serializer v) <= 2040)
+
 val value_spec_parser : P.spec_parser value_t
 
 val value_spec_serializer : P.spec_serializer value_spec_parser
+
+val value_spec_parser_injective (b1 b2: _) : Lemma
+  (requires (match value_spec_parser b1, value_spec_parser b2 with
+  | Some (v1, n1), Some (v2, n2) -> v1 == v2
+  | _ -> False
+  ))
+  (ensures (match value_spec_parser b1, value_spec_parser b2 with
+  | Some (v1, n1), Some (v2, n2) -> (n1 <: nat) == n2 /\ Seq.slice b1 0 n1 == Seq.slice b2 0 n2
+  | _ -> True
+  ))
+
+val value_spec_parser_strong_prefix (b1 b2: _) : Lemma
+  (requires (
+    match value_spec_parser b1 with
+    | Some (_, n1) -> n1 <= Seq.length b2 /\ Seq.slice b1 0 n1 == Seq.slice b2 0 n1
+    | _ -> False
+  ))
+  (ensures (
+    match value_spec_parser b1, value_spec_parser b2 with
+    | Some (v1, _), Some (v2, _) -> v1 == v2
+    | _ -> False
+  ))
+
+/// This is an ad hoc bound due to a bound on Blake hashable inputs
+/// FIXME: this bound is necessary because QuackyDucky expects a constant bound on abstract types
+val serialized_value_length (v:value_t)
+  : Lemma (Seq.length (value_spec_serializer v) <= 2040)
 
 val vget_args_spec_parser : P.spec_parser vget_args_t
 
